TM/Combinators/Match.v
@@ -12,11 +12,11 @@ Section Match.
   Variable F' : finType.
   Variable pMf : F -> pTM sig F' n.
 
-  Notation "'M1'" := (projT1 pM1) (only parsing).
-  Notation "'p1'":= (projT2 pM1) (only parsing).
+  Notation "'M1'" := (projT1 pM1).
+  Notation "'p1'":= (projT2 pM1).
 
-  Notation "'Mf' f" := (projT1 (pMf f)) (only parsing, at level 10).
-  Notation "'p2' f" := (projT2 (pMf f)) (only parsing, at level 10).
+  Notation "'Mf' f" := (projT1 (pMf f)) (at level 10).
+  Notation "'p2' f" := (projT2 (pMf f)) (at level 10).
 
   Definition Match_trans :
     (TM.states M1 + { f : F & TM.states (Mf f) }) * Vector.t (option sig) n ->
@@ -46,7 +46,6 @@ Section Match.
       start := inl (start M1);
     |}.
 
-  
   Definition Match_p : (states Match) -> F' :=
     fun q => match q with
           | inl q => p2 (p1 q) (start (Mf (p1 q))) (* Canonical value *)
@@ -54,6 +53,7 @@ Section Match.
           end.
   
   Definition MATCH := (Match; Match_p).
+
   
 
   (** Lift configurations of [M1] to configurations of [Match] *)
@@ -67,15 +67,15 @@ Section Match.
 
   (** Lifted Steps of [M1] are compatible with steps in [M1], for non-halting states *)
   Lemma step_comp_liftL (c : mconfig sig (states M1) n) :
-    halt (cstate c) = false -> lift_confL (step c) = step (lift_confL c).
+    haltConf c = false -> step (lift_confL c) = lift_confL (step c).
   Proof.
-    destruct c; cbn. unfold lift_confL, step. cbn. intros H. rewrite H.
+    unfold lift_confL, step, haltConf. cbn. destruct c as [q t]; cbn in *. intros H. rewrite H.
     destruct (trans _) eqn:E. cbn. reflexivity.
   Qed.
 
   (** Lifted steps of case-machines [Mf f] are compatible with steps in [Mf f] *)
   Lemma step_comp_liftR f (c : mconfig sig (states (Mf f)) n) :
-    lift_confR (step c) = step (lift_confR c).
+    step (lift_confR c) = lift_confR (step c).
   Proof.
     destruct c. unfold lift_confR, step. cbn.
     destruct (trans _) eqn:E. cbn. reflexivity.
@@ -101,7 +101,7 @@ Section Match.
   (** The "nop" transition jumps from a halting configuration of [M1] to the initial configuration of the corresponding case-machine. *)
   Lemma step_nop_transition (c : mconfig sig (states M1) n) :
     haltConf c = true ->
-    step (lift_confL c) = lift_confR (initc (Mf (p1 (cstate c))) (ctapes c)).
+     step (lift_confL c) = lift_confR (initc (Mf (p1 (cstate c))) (ctapes c)).
   Proof.
     intros Halt.
     unfold lift_confL, lift_confR. cbn. unfold haltConf in Halt.
@@ -124,7 +124,7 @@ Section Match.
     loopM (k1 + (1 + k2)) (initc Match t) = Some (lift_confR c2).
   Proof.
     intros HLoop1 HLoop2. unfold loopM in *.
-    apply loop_merge with (p := halt_liftL) (a2 := lift_confL c1).
+    apply loop_merge with (h := halt_liftL) (c2 := lift_confL c1).
     - apply halt_conf_liftL.
     - rewrite lift_initc.
       apply loop_lift with (h := haltConf (M := M1)) (f := step (M := M1)).
@@ -134,146 +134,13 @@ Section Match.
     - (* execute one step *)
       change (loop (1 + k2) (step (M:=Match)) (haltConf (M:=Match)) (lift_confL c1))
         with (loop k2 (step (M:=Match)) (haltConf (M:=Match)) (step (lift_confL c1))).
-      eapply loop_lift with (lift := lift_confR (f := p1 (cstate c1))) (g := step (M := Match)) (hlift := haltConf (M := Match)) in HLoop2.
-      + rewrite <- HLoop2. f_equal. apply step_nop_transition. apply (loop_fulfills_p HLoop1).
-      + intros. cbn. reflexivity.
+      rewrite step_nop_transition by apply (loop_fulfills_p HLoop1).
+      eapply loop_lift with (lift := lift_confR (f := p1 (cstate c1))) (f' := step (M := Match)) (h' := haltConf (M := Match)) in HLoop2.
+      + apply HLoop2.
+      + intros. cbn. now destruct x.
       + intros. apply step_comp_liftR.
   Qed.
 
-
-  (** The unlift functions map the configuration/state of [Match] to the corresponding states of either [M1] or some [Mf f]. *)
-  Definition unlift_confL : mconfig sig (states Match) n -> option (mconfig sig (states M1) n) :=
-    fun c =>
-      match (cstate c) with
-      | inl q => Some (mk_mconfig q (ctapes c))
-      | inr _ => None
-      end.
-
-  Definition unlift_confR (f : F) : mconfig sig (states Match) n -> option (mconfig sig (states (Mf f)) n).
-  Proof.
-    cbn in *.
-    refine (fun c =>
-              match (cstate c) with
-              | inl _ => None
-              | inr q => _
-              end).
-    destruct q as [y q]. decide (y = f) as [e | _].
-    - refine (Some (mk_mconfig _ (ctapes c))).
-      rewrite <- e. apply q.
-    - apply None.
-  Defined.
-
-
-  (** The lift and unlift functions are retracts. *)
-  Lemma retract_L (c : mconfig sig (states Match) n) (c' : mconfig sig (states M1) n) :
-    unlift_confL c = Some c' -> c = lift_confL c'.
-  Proof.
-    destruct c as [q t]. unfold unlift_confL, lift_confL. cbn. intros H.
-    destruct q as [ q | ?]; inv H. cbn. reflexivity.
-  Qed.
-
-  Lemma retract_L' (f : F) (c : mconfig sig (states M1) n) :
-    unlift_confL (lift_confL c) = Some c.
-  Proof. destruct c as [q t]. unfold unlift_confL, lift_confL. cbn. reflexivity. Qed.
-  
-
-  Lemma retract_R (f : F) (c : mconfig sig (states Match) n) (c' : mconfig sig (states (Mf f)) n) :
-    unlift_confR f c = Some c' -> c = lift_confR c'.
-  Proof.
-    destruct c as [q t]. unfold unlift_confR, lift_confR. cbn. intros H.
-    destruct q as [ q | [y q]]. inv H.
-    decide (y = f) as [ -> | ?]; inv H.
-    cbn. reflexivity.
-  Qed.
-
-  Lemma retract_R' (f : F) (c : mconfig sig (states (Mf f)) n) :
-    unlift_confR f (lift_confR c) = Some c.
-  Proof.
-    destruct c as [q t]. unfold unlift_confR, lift_confR. cbn. decide (f=f); try tauto.
-    f_equal. f_equal.
-    erewrite <- Eqdep_dec.eq_rect_eq_dec; auto. apply eqType_dec.
-  Qed.
-
-
-  (** If the configuration [c] of [Match] corresponds to the non-halting configuration [c'] of [M1], then [Match] simulates the step a step from [c']. *)
-  Lemma unlift_confL_step (c : mconfig sig (states Match) n) (c' : mconfig sig (states M1) n) :
-    unlift_confL c = Some c' ->
-    haltConf c' = false ->
-    unlift_confL (step c) = Some (step c').
-  Proof.
-    intros HUnlift HHalt. unfold haltConf in HHalt.
-    destruct c as [q t]. cbn in *.
-    unfold unlift_confL in *. cbn in *.
-    destruct q; inv HUnlift.
-    unfold step; cbn in *. rewrite HHalt.
-    now destruct trans.
-  Qed.
-  
-  (** If the configuration [c] of [Match] corresponds to the non-halting configuration [c'] of [Mf f], then [Match] simulates the step a step from [c']. *)
-  Lemma unlift_confR_step f (c : mconfig sig (states Match) n) (c' : mconfig sig (states (Mf f)) n) :
-    unlift_confR f c = Some c' ->
-    haltConf c' = false ->
-    unlift_confR f (step c) = Some (step c').
-  Proof.
-    intros HUnlift HHalt.
-    destruct c as [q t]. cbn in *.
-    unfold step. cbn [cstate ctapes].
-    unfold unlift_confR in *. cbn [cstate ctapes] in HUnlift.
-    destruct q as [q | [y q]]. inv HUnlift.
-    decide (y=f) as [ -> | _].
-    - inv HUnlift. cbn in *.
-      destruct (trans (q, current_chars t)) as [nextq acts] eqn:E. cbn.
-      decide (f=f); try tauto. f_equal. f_equal.
-      erewrite <- Eqdep_dec.eq_rect_eq_dec; auto. apply eqType_dec.
-    - inv HUnlift.
-  Qed.
-
-
-  (** Is the configuration [c] of [Match] a halting state of [M1] or no state of [M1] at all? *)
-  Definition halt_unliftL : mconfig sig (states Match) n -> bool :=
-    fun c =>
-      match unlift_confL c with
-      | Some c' => haltConf c'
-      | None => default (* this is no configuration of [M1] *)
-      end.
-
-
-  Lemma halt_comp_unliftL (c : mconfig sig (states Match) n) :
-    halt_unliftL c = false ->
-    haltConf c = false.
-  Proof.
-    destruct c as [q t]. cbn. unfold halt_unliftL, unlift_confL. cbn.
-    intros H. destruct q as [q | ?]; cbn in *; auto.
-  Qed.
-
-  (** If [c] is a state of [Match] that corresponds to a state [c'] of [M1], then the values of the halting functions are compatible. *)
-  Lemma halt_sim_unliftL (c : mconfig sig (states Match) n) (c' : mconfig sig (states M1) n) :
-    unlift_confL c = Some c' ->
-    haltConf c' = halt_unliftL c.
-  Proof. intros -> % retract_L. cbn. now destruct c'. Qed.
-
-
-  (* XXX: Has it to be true or false? *)
-  Arguments default : simpl never.
-
-  Definition halt_unliftR (f : F) : mconfig sig (states Match) n -> bool :=
-    fun c =>
-      match unlift_confR f c with
-      | Some c' => haltConf c'
-      | None => default (* this is no configuration of [Mf f] *)
-      end.
-
-  Lemma halt_sim_unliftR (f : F) (c : mconfig sig (states Match) n) (c' : mconfig sig (states (Mf f)) n) :
-    unlift_confR f c = Some c' ->
-    haltConf c' = halt_unliftR f c.
-  Proof.
-    intros -> % retract_R.
-    unfold halt_unliftR, unlift_confR. cbn.
-    decide (f=f); try tauto.
-    destruct c'; cbn. f_equal. f_equal.
-    erewrite <- Eqdep_dec.eq_rect_eq_dec; auto. apply eqType_dec.
-  Qed.
-    
 
   (** The [Match] machine must take the "nop" action if it is in a final state of [M1]. *)
   Lemma step_nop_split (k2 : nat) (c2 : mconfig sig (states M1) n) (outc : mconfig sig (states Match) n) :
@@ -288,39 +155,33 @@ Section Match.
     destruct k2 as [ | k2'].
     - inv HLoop2.
     - exists k2'. cbn in HLoop2.
-      replace (step (lift_confL c2)) with (lift_confR (initc (Mf (p1 (cstate c2))) (ctapes c2))) in HLoop2; cycle 1.
-      { cbv [step]. cbn -[tape_move_multi]. rewrite HHalt. rewrite tape_move_null_action. reflexivity. }
-      apply loop_unlift with (unlift := @unlift_confR (p1 (cstate c2)))
-                              (a := initc (Mf (p1 (cstate c2))) (ctapes c2))
-                              (f := step (M := Mf (p1 (cstate c2))))
-                              (p := haltConf (M := Mf (p1 (cstate c2)))) in HLoop2
-        as (c2'&HLoop2&HLoop2').
-      + apply retract_R in HLoop2' as ->.  exists c2'. repeat split; auto.
-      + intros. now apply unlift_confR_step.
-      + intros ? ? -> % retract_R. cbn. now destruct a.
-      + apply retract_R'.
+      rewrite step_nop_transition in HLoop2 by assumption.
+      apply loop_unlift with
+          (f := step (M := Mf (p1 (cstate c2))))
+          (h := haltConf (M := Mf (p1 (cstate c2)))) in HLoop2 as
+          (c2'&HLoop2&->).
+      + exists c2'. repeat split. exact HLoop2.
+      + intros. reflexivity.
+      + intros. apply step_comp_liftR.
   Qed.
 
 
-  Lemma Match_split i t (outc : mconfig sig (states Match) n) :
-    loopM i (initc Match t) = Some outc ->
+  Lemma Match_split k t (outc : mconfig sig (states Match) n) :
+    loopM k (initc Match t) = Some outc ->
     exists k1 (c1 : mconfig sig (states M1) n) k2 (c2 : mconfig sig (states (Mf (p1 (cstate c1)))) n),
       loopM k1 (initc M1 t) = Some c1 /\
       loopM k2 (initc (Mf (p1 (cstate c1))) (ctapes c1)) = Some c2 /\
       outc = lift_confR c2.
   Proof.
     unfold loopM. intros H.
-    apply loop_split with (p := halt_unliftL) in H as (k1&c1&k2&HLoop1&HLoop2&->).
-    - eapply loop_unlift with (unlift := unlift_confL) (a := initc M1 t) (f := step (M := M1)) (p := haltConf (M := M1)) in HLoop1
-        as (c1'&HLoop1&HLoop1').
-      + apply retract_L in HLoop1' as ->.
-        move HLoop2 at bottom.
-        apply step_nop_split in HLoop2 as (k2'&c2'&->&HLoop2&->). 2: exact (loop_fulfills_p HLoop1).
+    apply loop_split with (h := halt_liftL) in H as (k1&c1&k2&HLoop1&HLoop2&_).
+    - rewrite lift_initc in HLoop1.
+      apply loop_unlift with (lift := lift_confL) (f := step (M := M1)) (h := haltConf (M := M1)) in HLoop1 as (c1'&HLoop1&->).
+      + apply step_nop_split in HLoop2 as (k2'&c2'&_&HLoop2&->). 2: now apply (loop_fulfills_p HLoop1).
         exists k1, c1', k2', c2'. auto.
-      + intros. now apply unlift_confL_step.
-      + intros. now apply halt_sim_unliftL.
-      + reflexivity.
-    - apply halt_comp_unliftL.
+      + intros. cbn. reflexivity.
+      + intros. now apply step_comp_liftL.
+    - apply halt_conf_liftL.
   Qed.
 
 
